Added seq, skip, if

ifs.c
@@ -1,0 +1,5 @@
+int main() {
+  if (1) {} else {}
+  if (0) {} else {}
+  return (17 / 2) / (15 / 5);
+}
