ch2o_bigstep/stores.v
@@ -1,3 +1,12 @@
-Require Export ZArith.
+From ch2o Require Export integer_coding.
 
 Definition store := list (option Z).
+
+Definition store_value_typed `{IntCoding K} oz :=
+  match oz with
+    None => True
+  | Some z => int_typed z sintT
+  end.
+
+Definition store_typed `{IntCoding K} st :=
+  Forall store_value_typed st.
