ifs_asm_safe.v
@@ -1,0 +1,22 @@
+From ch2o_compcert Require Export ifs_ch2o_safe ifs_csyntaxgen_simplified ch2o_compcertc_lp64 compcertc_compiler.
+
+Lemma ifs_compcertc_safe: compcertc_safe_program (λ z, z = 2) prog.
+Proof.
+apply soundness with (2:=ifs_ch2o_safe).
+econstructor.
+- apply δ_main.
+- apply init_mem_ok.
+  reflexivity.
+- reflexivity.
+- reflexivity.
+- repeat constructor; (unfold int_lower || unfold int_upper); simpl; lia.
+Qed.
+
+Theorem ifs_asm_safe tp:
+  transf_c_program prog = OK tp →
+  asm_program_satisfies_spec tp (satisfies_postcondition (λ z, z = 2)).
+Proof.
+intros.
+apply transf_c_program_safe with (1:=H).
+apply ifs_compcertc_safe.
+Qed.
