ifs_ch2o.v
@@ -1,0 +1,23 @@
+Require Export String.
+Require Export ch2o.abstract_c.frontend.
+
+Local Open Scope string_scope.
+
+Definition decls: list (string * decl) :=
+  [("main",
+    FunDecl [] (CTFun [] (CTInt (CIntType None CIntRank)))
+      (CSComp
+        (CSIf (CEConst (CIntType (Some Signed) CIntRank) 1) (CSScope CSSkip)
+          (CSScope CSSkip))
+        (CSComp
+          (CSIf (CEConst (CIntType (Some Signed) CIntRank) 0)
+            (CSScope CSSkip) (CSScope CSSkip))
+          (CSReturn
+            (Some
+              (CEBinOp (ArithOp DivOp)
+                (CEBinOp (ArithOp DivOp)
+                  (CEConst (CIntType (Some Signed) CIntRank) 17)
+                  (CEConst (CIntType (Some Signed) CIntRank) 2))
+                (CEBinOp (ArithOp DivOp)
+                  (CEConst (CIntType (Some Signed) CIntRank) 15)
+                  (CEConst (CIntType (Some Signed) CIntRank) 5))))))))].
