ifs_ch2o_core_c.v
@@ -1,0 +1,86 @@
+From ch2o_compcert Require Export ch2o_lp64 ifs_ch2o.
+From ch2o Require Import stringmap frontend_sound.
+
+Local Open Scope string_scope.
+
+Definition alloc_program_result: frontend_state K.
+Proof.
+set (a:=alloc_program (K:=K) decls ∅).
+assert (match a with inl _ => False | inr _ => True end). { exact I. }
+destruct a. { elim H. }
+destruct p.
+exact f.
+Defined.
+
+Definition Γ: env K := to_env alloc_program_result.
+Definition δ: funenv K := to_funenv alloc_program_result.
+Definition m0: mem K := to_mem alloc_program_result.
+Definition S0 := initial_state m0 "main" [].
+
+Goal env_t Γ = ∅.
+Proof.
+reflexivity.
+Qed.
+
+Goal stringmap_to_list (env_f Γ) = [("main", ([], sintT%T))].
+reflexivity.
+Qed.
+
+(*
+
+Compute stringmap_to_list δ.
+
+*)
+
+Goal stringmap_to_list δ = [
+  ("main",
+   if{# intV{sintT} 1} skip else skip ;;
+   if{# intV{sintT} 0} skip else skip ;;
+   ret
+     (cast{sintT%T} (
+        # intV{sintT} 17 / # intV{sintT} 2 /
+        (# intV{sintT} 15 / # intV{sintT} 5))))
+].
+Proof.
+reflexivity.
+Qed.
+
+Lemma δ_main: δ !! ("main": funname) = Some (
+   if{# intV{sintT} 1} skip else skip ;;
+   if{# intV{sintT} 0} skip else skip ;;
+   ret
+     (cast{sintT%T} (
+        # intV{sintT} 17 / # intV{sintT} 2 /
+        (# intV{sintT} 15 / # intV{sintT} 5))) : stmt K).
+Proof.
+reflexivity.
+Qed.
+
+Goal m0 = ∅.
+Proof.
+reflexivity.
+Qed.
+
+Goal S0 = State [] (Call "main" []) m0.
+Proof.
+reflexivity.
+Qed.
+
+Lemma alloc_program_eq: alloc_program decls empty = mret () alloc_program_result.
+Proof.
+reflexivity.
+Qed.
+
+Lemma Γ_valid: ✓ Γ.
+Proof.
+apply alloc_program_valid with (1:=alloc_program_eq).
+Qed.
+
+Lemma δ_valid: ✓{Γ,'{m0}} δ.
+Proof.
+apply alloc_program_valid with (1:=alloc_program_eq).
+Qed.
+
+Lemma m0_valid: ✓{Γ} m0.
+apply alloc_program_valid with (1:=alloc_program_eq).
+Qed.
